---
title: Pascal's Identity
author: ''
date: '2021-02-27'
slug: pascal-s-identity
categories: []
tags: []
subtitle: ''
summary: "Pascal's Identity expresses a binomial coefficient in $n$ as the sum of two binomial coefficients in $n-1$."
authors: []
lastmod: '2021-02-27T16:14:39-05:00'
featured: no
image:
  caption: ''
  focal_point: ''
  preview_only: no
projects: []
math: true
draft: true
---
**Pascal's Identity**, also known as Pascal's Rule, expresses a binomial coefficient in $n$ as the sum of two binomial coefficients in $n-1$. 
```{python, results='asis', echo=FALSE}
import pascal as ML
```

```{theorem, name="Pascal's Identity"}
For integers $n$ and $k$, where $k \le n$, Pascal's Identity is given by the identity

\begin{equation}
{ n \choose k} = {n-1 \choose k-1} + {n-1 \choose k}
\end{equation}
```

### Proof

\begin{aligned}
{n \choose k} = & \ \ { n \choose k}      \\[1em]
              = & \ \ \frac{n!}{k!(n-k)!} \\[1em]
              = & \ \ \frac{(n-1)!}{(k-1)!(n-1-k)!} \left[ \frac{n}{(n-k)k} \right] \\[1em]
              = & \ \ \frac{(n-1)!}{(k-1)!(n-1-k)!} \left[ \frac{1}{(n-k)}+ \frac{1}{k}\right] \\[1em]
              = & \ \ \left[ \frac{(n-1)!}{(k-1)!(n-k)!} + \frac{(n-1)!}{k!(n-1-k)!} \right] \\[1em]
              = & \ \ {n-1 \choose k-1} + {n-1 \choose k} \\[1em]
                & & \qedsymbol
\end{aligned}

When using Pascal's Triangle, the apparent relationship between these combinations are apparent. For example, suppose $n=5$ and $k=2$, then Pascal's Identity states

\begin{aligned}
\bluebox{ ${ 5 \choose 2}$ } = \ \ & \greenbox{ ${5-1 \choose 2-1}$ } + \greenbox{ ${5-1 \choose 2}$ } \\[1em]
                         = \ \ & \greenbox{ ${4 \choose 1}$ } + \greenbox{ ${4 \choose 2}$ }. \\[1em]
\end{aligned}

The pattern is clear in Pascal's Triangle.

```{python, results='asis', echo=FALSE}
print(ML.pascals_triangle(6, combo="TRUE",
    highlight=[(4,1,'green'), (4,2,'green'), (5,2,'blue')]))
```
